Added type abstraction and application

Expression.thy
@@ -10,6 +10,30 @@ datatype expr =
 | Proj expr nat
 | Inj nat "type list" expr
 | Case expr "expr list"
+| TyAbs expr
+| TyApp expr type
+
+primrec incr\<^sub>t\<^sub>e :: "nat \<Rightarrow> expr \<Rightarrow> expr" where
+  "incr\<^sub>t\<^sub>e x (Var y) = Var y"
+| "incr\<^sub>t\<^sub>e x (Abs t e) = Abs (incr\<^sub>t\<^sub>t x t) (incr\<^sub>t\<^sub>e x e)"
+| "incr\<^sub>t\<^sub>e x (App e\<^sub>1 e\<^sub>2) = App (incr\<^sub>t\<^sub>e x e\<^sub>1) (incr\<^sub>t\<^sub>e x e\<^sub>2)"
+| "incr\<^sub>t\<^sub>e x (Rec fs) = Rec (map (incr\<^sub>t\<^sub>e x) fs)"
+| "incr\<^sub>t\<^sub>e x (Proj e l) = Proj (incr\<^sub>t\<^sub>e x e) l"
+| "incr\<^sub>t\<^sub>e x (Inj l ts e) = Inj l (map (incr\<^sub>t\<^sub>t x) ts) (incr\<^sub>t\<^sub>e x e)"
+| "incr\<^sub>t\<^sub>e x (Case e cs) = Case (incr\<^sub>t\<^sub>e x e) (map (incr\<^sub>t\<^sub>e x) cs)"
+| "incr\<^sub>t\<^sub>e x (TyAbs e) = TyAbs (incr\<^sub>t\<^sub>e (Suc x) e)"
+| "incr\<^sub>t\<^sub>e x (TyApp e t) = TyApp (incr\<^sub>t\<^sub>e x e) (incr\<^sub>t\<^sub>t x t)"
+
+primrec subst\<^sub>t\<^sub>e :: "nat \<Rightarrow> type \<Rightarrow> expr \<Rightarrow> expr" where
+  "subst\<^sub>t\<^sub>e x t' (Var y) = Var y"
+| "subst\<^sub>t\<^sub>e x t' (Abs t e) = Abs (subst\<^sub>t\<^sub>t x t' t) (subst\<^sub>t\<^sub>e x t' e)"
+| "subst\<^sub>t\<^sub>e x t' (App e\<^sub>1 e\<^sub>2) = App (subst\<^sub>t\<^sub>e x t' e\<^sub>1) (subst\<^sub>t\<^sub>e x t' e\<^sub>2)"
+| "subst\<^sub>t\<^sub>e x t' (Rec fs) = Rec (map (subst\<^sub>t\<^sub>e x t') fs)"
+| "subst\<^sub>t\<^sub>e x t' (Proj e l) = Proj (subst\<^sub>t\<^sub>e x t' e) l"
+| "subst\<^sub>t\<^sub>e x t' (Inj l ts e) = Inj l (map (subst\<^sub>t\<^sub>t x t') ts) (subst\<^sub>t\<^sub>e x t' e)"
+| "subst\<^sub>t\<^sub>e x t' (Case e cs) = Case (subst\<^sub>t\<^sub>e x t' e) (map (subst\<^sub>t\<^sub>e x t') cs)"
+| "subst\<^sub>t\<^sub>e x t' (TyAbs e) = TyAbs (subst\<^sub>t\<^sub>e (Suc x) (incr\<^sub>t\<^sub>t 0 t') e)"
+| "subst\<^sub>t\<^sub>e x t' (TyApp e t) = TyApp (subst\<^sub>t\<^sub>e x t' e) (subst\<^sub>t\<^sub>t x t' t)"
 
 primrec incr\<^sub>e\<^sub>e :: "nat \<Rightarrow> expr \<Rightarrow> expr" where
   "incr\<^sub>e\<^sub>e x (Var y) = Var (if x \<le> y then Suc y else y)"
@@ -19,6 +43,8 @@ primrec incr\<^sub>e\<^sub>e :: "nat \<Rightarrow> expr \<Rightarrow> expr" wher
 | "incr\<^sub>e\<^sub>e x (Proj e l) = Proj (incr\<^sub>e\<^sub>e x e) l"
 | "incr\<^sub>e\<^sub>e x (Inj l ts e) = Inj l ts (incr\<^sub>e\<^sub>e x e)"
 | "incr\<^sub>e\<^sub>e x (Case e cs) = Case (incr\<^sub>e\<^sub>e x e) (map (incr\<^sub>e\<^sub>e (Suc x)) cs)"
+| "incr\<^sub>e\<^sub>e x (TyAbs e) = TyAbs (incr\<^sub>e\<^sub>e x e)"
+| "incr\<^sub>e\<^sub>e x (TyApp e t) = TyApp (incr\<^sub>e\<^sub>e x e) t"
 
 primrec subst\<^sub>e\<^sub>e :: "nat \<Rightarrow> expr \<Rightarrow> expr \<Rightarrow> expr" where
   "subst\<^sub>e\<^sub>e x e' (Var y) = (if x = y then e' else Var (if x < y then y - 1 else y))"
@@ -28,6 +54,8 @@ primrec subst\<^sub>e\<^sub>e :: "nat \<Rightarrow> expr \<Rightarrow> expr \<Ri
 | "subst\<^sub>e\<^sub>e x e' (Proj e l) = Proj (subst\<^sub>e\<^sub>e x e' e) l"
 | "subst\<^sub>e\<^sub>e x e' (Inj l ts e) = Inj l ts (subst\<^sub>e\<^sub>e x e' e)"
 | "subst\<^sub>e\<^sub>e x e' (Case e cs) = Case (subst\<^sub>e\<^sub>e x e' e) (map (subst\<^sub>e\<^sub>e (Suc x) (incr\<^sub>e\<^sub>e 0 e')) cs)"
+| "subst\<^sub>e\<^sub>e x e' (TyAbs e) = TyAbs (subst\<^sub>e\<^sub>e x (incr\<^sub>t\<^sub>e 0 e') e)"
+| "subst\<^sub>e\<^sub>e x e' (TyApp e t) = TyApp (subst\<^sub>e\<^sub>e x e' e) t"
 
 primrec is_value :: "expr \<Rightarrow> bool" 
     and is_value_f :: "expr list \<Rightarrow> bool" where
@@ -38,6 +66,8 @@ primrec is_value :: "expr \<Rightarrow> bool"
 | "is_value (Proj e l) = False"
 | "is_value (Inj l ts e) = is_value e"
 | "is_value (Case e cs) = False"
+| "is_value (TyAbs e) = True"
+| "is_value (TyApp e t) = False"
 | "is_value_f [] = True"
 | "is_value_f (e # fs) = (is_value e \<and> is_value_f fs)"
 
