Stack.thy
@@ -9,30 +9,35 @@ datatype frame =
 | SProj nat
 | SInj nat "type list"
 | SCase "expr list" 
+| STyApp type 
 
-inductive typecheck_frame :: "type list \<Rightarrow> frame \<Rightarrow> type \<Rightarrow> type \<Rightarrow> bool" (infix "\<turnstile> _ : _ \<rightarrow>" 60) where
-  tc_sapp1 [simp]: "\<Gamma> \<turnstile> e : t\<^sub>1 \<Longrightarrow> \<Gamma> \<turnstile> SApp1 e : Arrow t\<^sub>1 t\<^sub>2 \<rightarrow> t\<^sub>2"
-| tc_sapp2 [simp]: "\<Gamma> \<turnstile> e : Arrow t\<^sub>1 t\<^sub>2 \<Longrightarrow> \<Gamma> \<turnstile> SApp2 e : t\<^sub>1 \<rightarrow> t\<^sub>2"
-| tc_srec [simp]: "\<Gamma> \<turnstile>\<^sub>f vs : vts \<Longrightarrow> \<Gamma> \<turnstile>\<^sub>f nvs : nvts \<Longrightarrow> 
-    \<Gamma> \<turnstile> SRec vs nvs : t \<rightarrow> Record (vts @ [t] @ nvts)"
-| tc_sproj [simp]: "lookup l ts = Some t \<Longrightarrow> \<Gamma> \<turnstile> SProj l : Record ts \<rightarrow> t"
-| tc_sinj [simp]: "lookup l ts = Some t \<Longrightarrow> \<Gamma> \<turnstile> SInj l ts : t \<rightarrow> Variant ts"
-| tc_scase [simp]: "\<Gamma> \<turnstile>\<^sub>c cs : ts \<rightarrow> t \<Longrightarrow> \<Gamma> \<turnstile> SCase cs : Variant ts \<rightarrow> t"
+inductive typecheck_frame :: "nat \<Rightarrow> type list \<Rightarrow> frame \<Rightarrow> type \<Rightarrow> type \<Rightarrow> bool" 
+    (infix ",_ \<turnstile> _ : _ \<rightarrow>" 60) where
+  tc_sapp1 [simp]: "\<Delta>,\<Gamma> \<turnstile> e : t\<^sub>1 \<Longrightarrow> \<Delta>,\<Gamma> \<turnstile> SApp1 e : Arrow t\<^sub>1 t\<^sub>2 \<rightarrow> t\<^sub>2"
+| tc_sapp2 [simp]: "\<Delta>,\<Gamma> \<turnstile> e : Arrow t\<^sub>1 t\<^sub>2 \<Longrightarrow> \<Delta>,\<Gamma> \<turnstile> SApp2 e : t\<^sub>1 \<rightarrow> t\<^sub>2"
+| tc_srec [simp]: "\<Delta>,\<Gamma> \<turnstile>\<^sub>f vs : vts \<Longrightarrow> \<Delta>,\<Gamma> \<turnstile>\<^sub>f nvs : nvts \<Longrightarrow> 
+    \<Delta>,\<Gamma> \<turnstile> SRec vs nvs : t \<rightarrow> Record (vts @ [t] @ nvts)"
+| tc_sproj [simp]: "lookup l ts = Some t \<Longrightarrow> \<Delta>,\<Gamma> \<turnstile> SProj l : Record ts \<rightarrow> t"
+| tc_sinj [simp]: "lookup l ts = Some t \<Longrightarrow> (\<forall>tt \<in> set ts. \<Delta> \<turnstile>\<^sub>k tt) \<Longrightarrow> 
+    \<Delta>,\<Gamma> \<turnstile> SInj l ts : t \<rightarrow> Variant ts"
+| tc_scase [simp]: "\<Delta>,\<Gamma> \<turnstile>\<^sub>c cs : ts \<rightarrow> t \<Longrightarrow> \<Delta>,\<Gamma> \<turnstile> SCase cs : Variant ts \<rightarrow> t"
+| tc_styapp [simp]: "\<Delta> \<turnstile>\<^sub>k t' \<Longrightarrow> \<Delta>,\<Gamma> \<turnstile> STyApp t' : Forall t \<rightarrow> subst\<^sub>t\<^sub>t 0 t' t"
 
-inductive_cases [elim]: "\<Gamma> \<turnstile> SApp1 e : t \<rightarrow> t'"
-inductive_cases [elim]: "\<Gamma> \<turnstile> SApp2 e : t \<rightarrow> t'"
-inductive_cases [elim]: "\<Gamma> \<turnstile> SRec vs nvs : t \<rightarrow> t'"
-inductive_cases [elim]: "\<Gamma> \<turnstile> SProj l : t \<rightarrow> t'"
-inductive_cases [elim]: "\<Gamma> \<turnstile> SInj l ts : t \<rightarrow> t'"
-inductive_cases [elim]: "\<Gamma> \<turnstile> SCase cs : t \<rightarrow> t'"
+inductive_cases [elim]: "\<Delta>,\<Gamma> \<turnstile> SApp1 e : t \<rightarrow> t'"
+inductive_cases [elim]: "\<Delta>,\<Gamma> \<turnstile> SApp2 e : t \<rightarrow> t'"
+inductive_cases [elim]: "\<Delta>,\<Gamma> \<turnstile> SRec vs nvs : t \<rightarrow> t'"
+inductive_cases [elim]: "\<Delta>,\<Gamma> \<turnstile> SProj l : t \<rightarrow> t'"
+inductive_cases [elim]: "\<Delta>,\<Gamma> \<turnstile> SInj l ts : t \<rightarrow> t'"
+inductive_cases [elim]: "\<Delta>,\<Gamma> \<turnstile> SCase cs : t \<rightarrow> t'"
+inductive_cases [elim]: "\<Delta>,\<Gamma> \<turnstile> STyApp tt : t \<rightarrow> t'"
 
-inductive typecheck_stack :: "type list \<Rightarrow> frame list \<Rightarrow> type \<Rightarrow> type \<Rightarrow> bool" 
-    (infix "\<turnstile>\<^sub>s _ : _ \<rightarrow>" 60) where
-  tcs_nil [simp]: "\<Gamma> \<turnstile>\<^sub>s [] : t \<rightarrow> t"
-| tcs_cons [simp]: "\<Gamma> \<turnstile>\<^sub>s s : t\<^sub>1 \<rightarrow> t\<^sub>2 \<Longrightarrow> \<Gamma> \<turnstile> f : t\<^sub>2 \<rightarrow> t\<^sub>3 \<Longrightarrow> \<Gamma> \<turnstile>\<^sub>s f # s : t\<^sub>1 \<rightarrow> t\<^sub>3"
+inductive typecheck_stack :: "nat \<Rightarrow> type list \<Rightarrow> frame list \<Rightarrow> type \<Rightarrow> type \<Rightarrow> bool" 
+    (infix ",_ \<turnstile>\<^sub>s _ : _ \<rightarrow>" 60) where
+  tcs_nil [simp]: "\<Delta>,\<Gamma> \<turnstile>\<^sub>s [] : t \<rightarrow> t"
+| tcs_cons [simp]: "\<Delta>,\<Gamma> \<turnstile>\<^sub>s s : t\<^sub>1 \<rightarrow> t\<^sub>2 \<Longrightarrow> \<Delta>,\<Gamma> \<turnstile> f : t\<^sub>2 \<rightarrow> t\<^sub>3 \<Longrightarrow> \<Delta>,\<Gamma> \<turnstile>\<^sub>s f # s : t\<^sub>1 \<rightarrow> t\<^sub>3"
 
-inductive_cases [elim]: "\<Gamma> \<turnstile>\<^sub>s [] : t \<rightarrow> t'"
-inductive_cases [elim]: "\<Gamma> \<turnstile>\<^sub>s f # s : t \<rightarrow> t'"
+inductive_cases [elim]: "\<Delta>,\<Gamma> \<turnstile>\<^sub>s [] : t \<rightarrow> t'"
+inductive_cases [elim]: "\<Delta>,\<Gamma> \<turnstile>\<^sub>s f # s : t \<rightarrow> t'"
 
 fun unfold :: "expr \<Rightarrow> frame list \<times> expr" 
 and unfold_f :: "expr list \<Rightarrow> expr list \<times> expr list \<times> frame list \<times> expr" where
@@ -60,6 +65,11 @@ and unfold_f :: "expr list \<Rightarrow> expr list \<times> expr list \<times> f
     if is_value e 
     then ([], Case e cs)
     else cons_fst (SCase cs) (unfold e))"
+| "unfold (TyAbs e) = ([], TyAbs e)"
+| "unfold (TyApp e t) = (
+    if is_value e 
+    then ([], TyApp e t)
+    else cons_fst (STyApp t) (unfold e))"
 | "unfold_f [] = undefined"
 | "unfold_f (e # fs) = (
     if is_value e
@@ -73,6 +83,7 @@ fun fold' :: "frame \<Rightarrow> expr \<Rightarrow> expr" where
 | "fold' (SProj l) e = Proj e l"
 | "fold' (SInj l ts) e = Inj l ts e"
 | "fold' (SCase cs) e = Case e cs"
+| "fold' (STyApp t) e = TyApp e t"
 
 fun fold :: "frame list \<Rightarrow> expr \<Rightarrow> expr" where
   "fold [] e = e"
@@ -83,22 +94,22 @@ lemma [simp]: "unfold e = (s, e') \<Longrightarrow> fold s e' = e"
   by (induction e and fs arbitrary: s e' and vs nvs s e' rule: unfold_unfold_f.induct) 
      (auto split: if_splits prod.splits)
 
-lemma [simp]: "\<Gamma> \<turnstile> f : t\<^sub>1 \<rightarrow> t\<^sub>2 \<Longrightarrow> \<Gamma> \<turnstile> e : t\<^sub>1 \<Longrightarrow> \<Gamma> \<turnstile> fold' f e : t\<^sub>2"
+lemma [simp]: "\<Delta>,\<Gamma> \<turnstile> f : t\<^sub>1 \<rightarrow> t\<^sub>2 \<Longrightarrow> \<Delta>,\<Gamma> \<turnstile> e : t\<^sub>1 \<Longrightarrow> \<Delta>,\<Gamma> \<turnstile> fold' f e : t\<^sub>2"
   by (induction \<Gamma> f t\<^sub>1 t\<^sub>2 rule: typecheck_frame.induct) simp_all
 
-lemma [simp]: "\<Gamma> \<turnstile>\<^sub>s s : t' \<rightarrow> t \<Longrightarrow> \<Gamma> \<turnstile> e : t' \<Longrightarrow> \<Gamma> \<turnstile> fold s e : t"
+lemma [simp]: "\<Delta>,\<Gamma> \<turnstile>\<^sub>s s : t' \<rightarrow> t \<Longrightarrow> \<Delta>,\<Gamma> \<turnstile> e : t' \<Longrightarrow> \<Delta>,\<Gamma> \<turnstile> fold s e : t"
   by (induction \<Gamma> s t' t rule: typecheck_stack.induct) simp_all
 
-lemma [simp]: "\<Gamma> \<turnstile> e : t \<Longrightarrow> unfold e = (s, e') \<Longrightarrow> \<exists>t'. (\<Gamma> \<turnstile>\<^sub>s s : t' \<rightarrow> t) \<and> (\<Gamma> \<turnstile> e' : t')"
-  and [simp]: "\<Gamma> \<turnstile>\<^sub>f fs : ts \<Longrightarrow> \<not> is_value_f fs \<Longrightarrow> unfold_f fs = (vs, nvs, s, e') \<Longrightarrow> 
-    \<exists>t t' vts nvts. ts = vts @ [t] @ nvts \<and> (\<Gamma> \<turnstile>\<^sub>s s : t' \<rightarrow> t) \<and> (\<Gamma> \<turnstile> e' : t') \<and> (\<Gamma> \<turnstile>\<^sub>f vs : vts) \<and> 
-      (\<Gamma> \<turnstile>\<^sub>f nvs : nvts)"
-  and [simp]: "\<Gamma> \<turnstile>\<^sub>c cs : ts \<rightarrow> t \<Longrightarrow> True"
-  proof (induction \<Gamma> e t and \<Gamma> fs ts arbitrary: s and vs nvs s 
+lemma [simp]: "\<Delta>,\<Gamma> \<turnstile> e : t \<Longrightarrow> unfold e = (s, e') \<Longrightarrow> \<exists>t'. (\<Delta>,\<Gamma> \<turnstile>\<^sub>s s : t' \<rightarrow> t) \<and> (\<Delta>,\<Gamma> \<turnstile> e' : t')"
+  and [simp]: "\<Delta>,\<Gamma> \<turnstile>\<^sub>f fs : ts \<Longrightarrow> \<not> is_value_f fs \<Longrightarrow> unfold_f fs = (vs, nvs, s, e') \<Longrightarrow> 
+    \<exists>t t' vts nvts. ts = vts @ [t] @ nvts \<and> (\<Delta>,\<Gamma> \<turnstile>\<^sub>s s : t' \<rightarrow> t) \<and> (\<Delta>,\<Gamma> \<turnstile> e' : t') \<and> 
+      (\<Delta>,\<Gamma> \<turnstile>\<^sub>f vs : vts) \<and> (\<Delta>,\<Gamma> \<turnstile>\<^sub>f nvs : nvts)"
+  and [simp]: "\<Delta>,\<Gamma> \<turnstile>\<^sub>c cs : ts \<rightarrow> t \<Longrightarrow> True"
+  proof (induction \<Delta> \<Gamma> e t and \<Delta> \<Gamma> fs ts arbitrary: s and vs nvs s 
          rule: typecheck_typecheck_fs_typecheck_cs.inducts)
   case (tc_var x \<Gamma> t)
     thus ?case by simp (metis tcs_nil typecheck_typecheck_fs_typecheck_cs.tc_var)
-  next case (tc_app \<Gamma> e\<^sub>1 t\<^sub>1 t\<^sub>2 e\<^sub>2)
+  next case (tc_app \<Delta> \<Gamma> e\<^sub>1 t\<^sub>1 t\<^sub>2 e\<^sub>2)
     thus ?case 
       proof (cases "is_value e\<^sub>1")
       case True note T = True
@@ -110,21 +121,22 @@ lemma [simp]: "\<Gamma> \<turnstile> e : t \<Longrightarrow> unfold e = (s, e') 
           next case False
             with tc_app True obtain s\<^sub>2 where "unfold e\<^sub>2 = (s\<^sub>2, e') \<and> s = SApp2 e\<^sub>1 # s\<^sub>2"
               by (auto split: prod.splits)
-            moreover with tc_app obtain t' where "(\<Gamma> \<turnstile>\<^sub>s s\<^sub>2 : t' \<rightarrow> t\<^sub>1) \<and> \<Gamma> \<turnstile> e' : t'" by fastforce
-            moreover with tc_app have "\<Gamma> \<turnstile>\<^sub>s SApp2 e\<^sub>1 # s\<^sub>2 : t' \<rightarrow> t\<^sub>2" by fastforce
+            moreover with tc_app obtain t' where "(\<Delta>,\<Gamma> \<turnstile>\<^sub>s s\<^sub>2 : t' \<rightarrow> t\<^sub>1) \<and> \<Delta>,\<Gamma> \<turnstile> e' : t'" 
+              by fastforce
+            moreover with tc_app have "\<Delta>,\<Gamma> \<turnstile>\<^sub>s SApp2 e\<^sub>1 # s\<^sub>2 : t' \<rightarrow> t\<^sub>2" by fastforce
             ultimately show ?thesis by fastforce
           qed
       next case False
         with tc_app obtain s\<^sub>1 where "unfold e\<^sub>1 = (s\<^sub>1, e') \<and> s = SApp1 e\<^sub>2 # s\<^sub>1" 
           by (auto split: prod.splits)
-        moreover with tc_app obtain t' where "(\<Gamma> \<turnstile>\<^sub>s s\<^sub>1 : t' \<rightarrow> Arrow t\<^sub>1 t\<^sub>2) \<and> \<Gamma> \<turnstile> e' : t'" 
+        moreover with tc_app obtain t' where "(\<Delta>,\<Gamma> \<turnstile>\<^sub>s s\<^sub>1 : t' \<rightarrow> Arrow t\<^sub>1 t\<^sub>2) \<and> \<Delta>,\<Gamma> \<turnstile> e' : t'" 
           by fastforce
-        moreover with tc_app have "\<Gamma> \<turnstile>\<^sub>s SApp1 e\<^sub>2 # s\<^sub>1 : t' \<rightarrow> t\<^sub>2" by fastforce
+        moreover with tc_app have "\<Delta>,\<Gamma> \<turnstile>\<^sub>s SApp1 e\<^sub>2 # s\<^sub>1 : t' \<rightarrow> t\<^sub>2" by fastforce
         ultimately show ?thesis by fastforce
       qed
-  next case (tc_abs t\<^sub>1 \<Gamma> e t\<^sub>2)
+  next case (tc_abs \<Delta> t\<^sub>1 \<Gamma> e t\<^sub>2)
     thus ?case by simp (metis tcs_nil typecheck_typecheck_fs_typecheck_cs.tc_abs)
-  next case (tc_rec \<Gamma> fs ts)
+  next case (tc_rec \<Delta> \<Gamma> fs ts)
     thus ?case 
       proof (cases "is_value_f fs")
       case True
@@ -133,11 +145,12 @@ lemma [simp]: "\<Gamma> \<turnstile> e : t \<Longrightarrow> unfold e = (s, e') 
         then obtain vs nvs ss ee' where F: "unfold_f fs = (vs, nvs, ss, ee')" 
           by (cases "unfold_f fs") simp_all
         with tc_rec False obtain t t' vts nvts where T: "ts = vts @ [t] @ nvts \<and> 
-            (\<Gamma> \<turnstile>\<^sub>s ss : t' \<rightarrow> t) \<and> (\<Gamma> \<turnstile> e' : t') \<and> (\<Gamma> \<turnstile>\<^sub>f vs : vts) \<and> \<Gamma> \<turnstile>\<^sub>f nvs : nvts" by fastforce
-        hence "\<Gamma> \<turnstile>\<^sub>s SRec vs nvs # ss : t' \<rightarrow> Record ts" using tc_srec by fastforce
+          (\<Delta>,\<Gamma> \<turnstile>\<^sub>s ss : t' \<rightarrow> t) \<and> (\<Delta>,\<Gamma> \<turnstile> e' : t') \<and> (\<Delta>,\<Gamma> \<turnstile>\<^sub>f vs : vts) \<and> \<Delta>,\<Gamma> \<turnstile>\<^sub>f nvs : nvts" 
+            by fastforce
+        hence "\<Delta>,\<Gamma> \<turnstile>\<^sub>s SRec vs nvs # ss : t' \<rightarrow> Record ts" using tc_srec by fastforce
         with tc_rec False F T show ?thesis by fastforce
       qed
-  next case (tc_proj \<Gamma> e ts l t)
+  next case (tc_proj \<Delta> \<Gamma> e ts l t)
     thus ?case
       proof (cases "is_value e")
       case True
@@ -145,12 +158,12 @@ lemma [simp]: "\<Gamma> \<turnstile> e : t \<Longrightarrow> unfold e = (s, e') 
       next case False
         with tc_proj obtain ss where "unfold e = (ss, e') \<and> s = SProj l # ss" 
           by (auto split: prod.splits)
-        moreover with tc_proj obtain t' where "(\<Gamma> \<turnstile>\<^sub>s ss : t' \<rightarrow> Record ts) \<and> (\<Gamma> \<turnstile> e' : t')" 
+        moreover with tc_proj obtain t' where "(\<Delta>,\<Gamma> \<turnstile>\<^sub>s ss : t' \<rightarrow> Record ts) \<and> (\<Delta>,\<Gamma> \<turnstile> e' : t')" 
           by fastforce
-        moreover with tc_proj have "\<Gamma> \<turnstile>\<^sub>s SProj l # ss : t' \<rightarrow> t" by fastforce
+        moreover with tc_proj have "\<Delta>,\<Gamma> \<turnstile>\<^sub>s SProj l # ss : t' \<rightarrow> t" by fastforce
         ultimately show ?thesis by fastforce
       qed
-  next case (tc_inj \<Gamma> e t l ts)
+  next case (tc_inj \<Delta> \<Gamma> e t l ts)
     thus ?case
       proof (cases "is_value e")
       case True
@@ -158,11 +171,11 @@ lemma [simp]: "\<Gamma> \<turnstile> e : t \<Longrightarrow> unfold e = (s, e') 
       next case False
         with tc_inj obtain s' where S: "unfold e = (s', e') \<and> s = SInj l ts # s'" 
           by (auto split: prod.splits)
-        with tc_inj obtain t' where "(\<Gamma> \<turnstile>\<^sub>s s' : t' \<rightarrow> t) \<and> (\<Gamma> \<turnstile> e' : t')" by fastforce
-        moreover with tc_inj S have "\<Gamma> \<turnstile>\<^sub>s s : t' \<rightarrow> Variant ts" using tc_sinj by fastforce
+        with tc_inj obtain t' where "(\<Delta>,\<Gamma> \<turnstile>\<^sub>s s' : t' \<rightarrow> t) \<and> (\<Delta>,\<Gamma> \<turnstile> e' : t')" by fastforce
+        moreover with tc_inj S have "\<Delta>,\<Gamma> \<turnstile>\<^sub>s s : t' \<rightarrow> Variant ts" using tc_sinj by fastforce
         ultimately show ?thesis by fastforce
       qed
-  next case (tc_case \<Gamma> e ts cs t)
+  next case (tc_case \<Delta> \<Gamma> e ts cs t)
     thus ?case
       proof (cases "is_value e")
       case True
@@ -170,25 +183,43 @@ lemma [simp]: "\<Gamma> \<turnstile> e : t \<Longrightarrow> unfold e = (s, e') 
       next case False
         with tc_case obtain s' where S: "unfold e = (s', e') \<and> s = SCase cs # s'" 
           by (auto split: prod.splits)
-        with tc_case obtain t' where T: "(\<Gamma> \<turnstile>\<^sub>s s' : t' \<rightarrow> Variant ts) \<and> (\<Gamma> \<turnstile> e' : t')" by fastforce
-        with tc_case S have "\<Gamma> \<turnstile>\<^sub>s s : t' \<rightarrow> t" using tc_scase by fastforce
+        with tc_case obtain t' where T: "(\<Delta>,\<Gamma> \<turnstile>\<^sub>s s' : t' \<rightarrow> Variant ts) \<and> (\<Delta>,\<Gamma> \<turnstile> e' : t')" 
+          by fastforce
+        with tc_case S have "\<Delta>,\<Gamma> \<turnstile>\<^sub>s s : t' \<rightarrow> t" using tc_scase by fastforce
         with T show ?thesis by fastforce
       qed
-  next case (tcf_cons \<Gamma> e tt fs ts)
+  next case (tc_tyabs \<Delta> \<Gamma> e t)
+    thus ?case by simp (metis tcs_nil typecheck_typecheck_fs_typecheck_cs.tc_tyabs)
+  next case (tc_tyapp \<Delta> \<Gamma> e t t')
+    thus ?case
+      proof (cases "is_value e")
+      case True
+        with tc_tyapp show ?thesis 
+          by simp (metis tcs_nil typecheck_typecheck_fs_typecheck_cs.tc_tyapp)
+      next case False
+        with tc_tyapp obtain s' where S: "unfold e = (s', e') \<and> s = STyApp t' # s'" 
+          by (auto split: prod.splits)
+        with tc_tyapp obtain tt where T: "(\<Delta>,\<Gamma> \<turnstile>\<^sub>s s' : tt \<rightarrow> Forall t) \<and> (\<Delta>,\<Gamma> \<turnstile> e' : tt)" 
+          by fastforce
+        with tc_tyapp have "\<Delta>,\<Gamma> \<turnstile>\<^sub>s STyApp t' # s' : tt \<rightarrow> subst\<^sub>t\<^sub>t 0 t' t" by fastforce
+        with S T show ?thesis by fastforce
+      qed
+  next case (tcf_cons \<Delta> \<Gamma> e tt fs ts)
     thus ?case
       proof (cases "is_value e")
       case True
         with tcf_cons obtain vs' where V: "unfold_f fs = (vs', nvs, s, e') \<and> vs = e # vs'" 
           by (cases "unfold_f fs") fastforce+
         moreover with tcf_cons True obtain t t' vts nvts where T: "ts = vts @ [t] @ nvts \<and> 
-          (\<Gamma> \<turnstile>\<^sub>s s : t' \<rightarrow> t) \<and> (\<Gamma> \<turnstile> e' : t') \<and> (\<Gamma> \<turnstile>\<^sub>f vs' : vts) \<and> \<Gamma> \<turnstile>\<^sub>f nvs : nvts" by fastforce
+          (\<Delta>,\<Gamma> \<turnstile>\<^sub>s s : t' \<rightarrow> t) \<and> (\<Delta>,\<Gamma> \<turnstile> e' : t') \<and> (\<Delta>,\<Gamma> \<turnstile>\<^sub>f vs' : vts) \<and> \<Delta>,\<Gamma> \<turnstile>\<^sub>f nvs : nvts" 
+            by fastforce
         moreover hence "tt # ts = (tt # vts) @ [t] @ nvts" by simp
-        moreover from tcf_cons V T have "\<Gamma> \<turnstile>\<^sub>f vs : tt # vts" by simp
+        moreover from tcf_cons V T have "\<Delta>,\<Gamma> \<turnstile>\<^sub>f vs : tt # vts" by simp
         ultimately show ?thesis by blast
       next case False
-        with tcf_cons obtain t' where "(\<Gamma> \<turnstile>\<^sub>s s : t' \<rightarrow> tt) \<and> \<Gamma> \<turnstile> e' : t'" by fastforce
-        moreover from tcf_cons False have "\<Gamma> \<turnstile>\<^sub>f vs : []" by simp
-        moreover from tcf_cons False have "\<Gamma> \<turnstile>\<^sub>f nvs : ts" by simp
+        with tcf_cons obtain t' where "(\<Delta>,\<Gamma> \<turnstile>\<^sub>s s : t' \<rightarrow> tt) \<and> \<Delta>,\<Gamma> \<turnstile> e' : t'" by fastforce
+        moreover from tcf_cons False have "\<Delta>,\<Gamma> \<turnstile>\<^sub>f vs : []" by simp
+        moreover from tcf_cons False have "\<Delta>,\<Gamma> \<turnstile>\<^sub>f nvs : ts" by simp
         ultimately show ?thesis by fastforce
       qed
   qed simp_all
