Type.thy
@@ -3,9 +3,57 @@ imports Main
 begin
 
 datatype type = 
-  Base
+  TyVar nat
 | Arrow type type
 | Record "type list"
 | Variant "type list"
+| Forall type
+
+primrec incr\<^sub>t\<^sub>t :: "nat \<Rightarrow> type \<Rightarrow> type" where
+  "incr\<^sub>t\<^sub>t x (TyVar y) = TyVar (if x \<le> y then Suc y else y)"
+| "incr\<^sub>t\<^sub>t x (Arrow t\<^sub>1 t\<^sub>2) = Arrow (incr\<^sub>t\<^sub>t x t\<^sub>1) (incr\<^sub>t\<^sub>t x t\<^sub>2)"
+| "incr\<^sub>t\<^sub>t x (Record ts) = Record (map (incr\<^sub>t\<^sub>t x) ts)"
+| "incr\<^sub>t\<^sub>t x (Variant ts) = Variant (map (incr\<^sub>t\<^sub>t x) ts)"
+| "incr\<^sub>t\<^sub>t x (Forall t) = Forall (incr\<^sub>t\<^sub>t (Suc x) t)"
+
+primrec subst\<^sub>t\<^sub>t :: "nat \<Rightarrow> type \<Rightarrow> type \<Rightarrow> type" where
+  "subst\<^sub>t\<^sub>t x t' (TyVar y) = (if x = y then t' else TyVar (if x < y then y - 1 else y))"
+| "subst\<^sub>t\<^sub>t x t' (Arrow t\<^sub>1 t\<^sub>2) = Arrow (subst\<^sub>t\<^sub>t x t' t\<^sub>1) (subst\<^sub>t\<^sub>t x t' t\<^sub>2)"
+| "subst\<^sub>t\<^sub>t x t' (Record ts) = Record (map (subst\<^sub>t\<^sub>t x t') ts)"
+| "subst\<^sub>t\<^sub>t x t' (Variant ts) = Variant (map (subst\<^sub>t\<^sub>t x t') ts)"
+| "subst\<^sub>t\<^sub>t x t' (Forall t) = Forall (subst\<^sub>t\<^sub>t (Suc x) (incr\<^sub>t\<^sub>t 0 t') t)"
+
+lemma [simp]: "y \<le> x \<Longrightarrow> incr\<^sub>t\<^sub>t y (incr\<^sub>t\<^sub>t x t) = incr\<^sub>t\<^sub>t (Suc x) (incr\<^sub>t\<^sub>t y t)"
+  by (induction t arbitrary: x y) simp_all
+
+lemma [simp]: "y \<le> x \<Longrightarrow> incr\<^sub>t\<^sub>t y o incr\<^sub>t\<^sub>t x = incr\<^sub>t\<^sub>t (Suc x) o incr\<^sub>t\<^sub>t y"
+  by rule simp
+
+lemma [simp]: "y \<le> x \<Longrightarrow> subst\<^sub>t\<^sub>t y (incr\<^sub>t\<^sub>t x t') (incr\<^sub>t\<^sub>t (Suc x) t) = incr\<^sub>t\<^sub>t x (subst\<^sub>t\<^sub>t y t' t)" 
+  by (induction t arbitrary: x y t') auto
+
+lemma [simp]: "y \<le> x \<Longrightarrow> subst\<^sub>t\<^sub>t y (incr\<^sub>t\<^sub>t x t') o incr\<^sub>t\<^sub>t (Suc x) = incr\<^sub>t\<^sub>t x o subst\<^sub>t\<^sub>t y t'" 
+  by rule simp
+
+lemma [simp]: "y \<le> x \<Longrightarrow> incr\<^sub>t\<^sub>t y (subst\<^sub>t\<^sub>t x t' t) = subst\<^sub>t\<^sub>t (Suc x) (incr\<^sub>t\<^sub>t y t') (incr\<^sub>t\<^sub>t y t)"
+  by (induction t arbitrary: x y t') auto
+
+lemma [simp]: "y \<le> x \<Longrightarrow> incr\<^sub>t\<^sub>t y \<circ> subst\<^sub>t\<^sub>t x t' = subst\<^sub>t\<^sub>t (Suc x) (incr\<^sub>t\<^sub>t y t') \<circ> incr\<^sub>t\<^sub>t y"
+  by rule simp
+
+lemma [simp]: "subst\<^sub>t\<^sub>t x t' (incr\<^sub>t\<^sub>t x t) = t"
+  proof (induction t arbitrary: x t')
+  case (Record ts)
+    thus ?case by (induction ts) simp_all
+  next case (Variant ts)
+    thus ?case by (induction ts) simp_all
+  qed simp_all
+
+lemma [simp]: "subst\<^sub>t\<^sub>t x t' o incr\<^sub>t\<^sub>t x = id"
+  by rule simp
+
+lemma [simp]: "y \<le> x \<Longrightarrow> 
+    subst\<^sub>t\<^sub>t x t\<^sub>1' (subst\<^sub>t\<^sub>t y t\<^sub>2' t) = subst\<^sub>t\<^sub>t y (subst\<^sub>t\<^sub>t x t\<^sub>1' t\<^sub>2') (subst\<^sub>t\<^sub>t (Suc x) (incr\<^sub>t\<^sub>t y t\<^sub>1') t)"
+  by (induction t arbitrary: x y t\<^sub>1' t\<^sub>2') auto
 
 end
