Typecheck.thy
@@ -1,78 +1,149 @@
 theory Typecheck
-imports Vector Expression
+imports Vector Expression Kindcheck
 begin
 
-inductive typecheck :: "type list \<Rightarrow> expr \<Rightarrow> type \<Rightarrow> bool" (infix "\<turnstile> _ :" 60) 
-      and typecheck_fs :: "type list \<Rightarrow> expr list \<Rightarrow> type list \<Rightarrow> bool" (infix "\<turnstile>\<^sub>f _ :" 60)
-      and typecheck_cs :: "type list \<Rightarrow> expr list \<Rightarrow> type list \<Rightarrow> type \<Rightarrow> bool" 
-    (infix "\<turnstile>\<^sub>c _ : _ \<rightarrow>" 60) where
-  tc_var [simp]: "lookup x \<Gamma> = Some t \<Longrightarrow> \<Gamma> \<turnstile> Var x : t"
-| tc_abs [simp]: "insert_at 0 t\<^sub>1 \<Gamma> \<turnstile> e : t\<^sub>2 \<Longrightarrow> \<Gamma> \<turnstile> Abs t\<^sub>1 e : Arrow t\<^sub>1 t\<^sub>2"
-| tc_app [simp]: "\<Gamma> \<turnstile> e\<^sub>1 : Arrow t\<^sub>1 t\<^sub>2 \<Longrightarrow> \<Gamma> \<turnstile> e\<^sub>2 : t\<^sub>1 \<Longrightarrow> \<Gamma> \<turnstile> App e\<^sub>1 e\<^sub>2 : t\<^sub>2"
-| tc_rec [simp]: "\<Gamma> \<turnstile>\<^sub>f fs : ts \<Longrightarrow> \<Gamma> \<turnstile> Rec fs : Record ts"
-| tc_proj [simp]: "\<Gamma> \<turnstile> e : Record ts \<Longrightarrow> lookup l ts = Some t \<Longrightarrow> \<Gamma> \<turnstile> Proj e l : t"
-| tc_inj [simp]: "\<Gamma> \<turnstile> e : t \<Longrightarrow> lookup l ts = Some t \<Longrightarrow> \<Gamma> \<turnstile> Inj l ts e : Variant ts"
-| tc_case [simp]: "\<Gamma> \<turnstile> e : Variant ts \<Longrightarrow> \<Gamma> \<turnstile>\<^sub>c cs : ts \<rightarrow> t \<Longrightarrow> \<Gamma> \<turnstile> Case e cs : t"
-| tcf_nil [simp]: "\<Gamma> \<turnstile>\<^sub>f [] : []"
-| tcf_cons [simp]: "\<Gamma> \<turnstile> e : t \<Longrightarrow> \<Gamma> \<turnstile>\<^sub>f fs : ts \<Longrightarrow> \<Gamma> \<turnstile>\<^sub>f e # fs : t # ts"
-| tcc_nil [simp]: "\<Gamma> \<turnstile>\<^sub>c [] : [] \<rightarrow> t"
-| tcc_cons [simp]: "insert_at 0 t' \<Gamma> \<turnstile> e : t \<Longrightarrow> \<Gamma> \<turnstile>\<^sub>c fs : ts \<rightarrow> t \<Longrightarrow> \<Gamma> \<turnstile>\<^sub>c e # fs : t' # ts \<rightarrow> t"
+inductive typecheck :: "nat \<Rightarrow> type list \<Rightarrow> expr \<Rightarrow> type \<Rightarrow> bool" (infix ",_ \<turnstile> _ :" 60) 
+      and typecheck_fs :: "nat \<Rightarrow> type list \<Rightarrow> expr list \<Rightarrow> type list \<Rightarrow> bool" (infix ",_ \<turnstile>\<^sub>f _ :" 60)
+      and typecheck_cs :: "nat \<Rightarrow> type list \<Rightarrow> expr list \<Rightarrow> type list \<Rightarrow> type \<Rightarrow> bool" 
+    (infix ",_ \<turnstile>\<^sub>c _ : _ \<rightarrow>" 60) where
+  tc_var [simp]: "lookup x \<Gamma> = Some t \<Longrightarrow> \<Delta>,\<Gamma> \<turnstile> Var x : t"
+| tc_abs [simp]: "\<Delta>,insert_at 0 t\<^sub>1 \<Gamma> \<turnstile> e : t\<^sub>2 \<Longrightarrow> \<Delta> \<turnstile>\<^sub>k t\<^sub>1 \<Longrightarrow> \<Delta>,\<Gamma> \<turnstile> Abs t\<^sub>1 e : Arrow t\<^sub>1 t\<^sub>2"
+| tc_app [simp]: "\<Delta>,\<Gamma> \<turnstile> e\<^sub>1 : Arrow t\<^sub>1 t\<^sub>2 \<Longrightarrow> \<Delta>,\<Gamma> \<turnstile> e\<^sub>2 : t\<^sub>1 \<Longrightarrow> \<Delta>,\<Gamma> \<turnstile> App e\<^sub>1 e\<^sub>2 : t\<^sub>2"
+| tc_rec [simp]: "\<Delta>,\<Gamma> \<turnstile>\<^sub>f fs : ts \<Longrightarrow> \<Delta>,\<Gamma> \<turnstile> Rec fs : Record ts"
+| tc_proj [simp]: "\<Delta>,\<Gamma> \<turnstile> e : Record ts \<Longrightarrow> lookup l ts = Some t \<Longrightarrow> \<Delta>,\<Gamma> \<turnstile> Proj e l : t"
+| tc_inj [simp]: "\<Delta>,\<Gamma> \<turnstile> e : t \<Longrightarrow> lookup l ts = Some t \<Longrightarrow> \<forall>tt \<in> set ts. \<Delta> \<turnstile>\<^sub>k tt \<Longrightarrow> 
+    \<Delta>,\<Gamma> \<turnstile> Inj l ts e : Variant ts"
+| tc_case [simp]: "\<Delta>,\<Gamma> \<turnstile> e : Variant ts \<Longrightarrow> \<Delta>,\<Gamma> \<turnstile>\<^sub>c cs : ts \<rightarrow> t \<Longrightarrow> \<Delta>,\<Gamma> \<turnstile> Case e cs : t"
+| tc_tyabs [simp]: "Suc \<Delta>,map (incr\<^sub>t\<^sub>t 0) \<Gamma> \<turnstile> e : t \<Longrightarrow> \<Delta>,\<Gamma> \<turnstile> TyAbs e : Forall t"
+| tc_tyapp [simp]: "\<Delta>,\<Gamma> \<turnstile> e : Forall t \<Longrightarrow> \<Delta> \<turnstile>\<^sub>k t' \<Longrightarrow> \<Delta>,\<Gamma> \<turnstile> TyApp e t' : subst\<^sub>t\<^sub>t 0 t' t"
+| tcf_nil [simp]: "\<Delta>,\<Gamma> \<turnstile>\<^sub>f [] : []"
+| tcf_cons [simp]: "\<Delta>,\<Gamma> \<turnstile> e : t \<Longrightarrow> \<Delta>,\<Gamma> \<turnstile>\<^sub>f fs : ts \<Longrightarrow> \<Delta>,\<Gamma> \<turnstile>\<^sub>f e # fs : t # ts"
+| tcc_nil [simp]: "\<Delta>,\<Gamma> \<turnstile>\<^sub>c [] : [] \<rightarrow> t"
+| tcc_cons [simp]: "\<Delta>,insert_at 0 t' \<Gamma> \<turnstile> e : t \<Longrightarrow> \<Delta>,\<Gamma> \<turnstile>\<^sub>c cs : ts \<rightarrow> t \<Longrightarrow> 
+    \<Delta>,\<Gamma> \<turnstile>\<^sub>c e # cs : t' # ts \<rightarrow> t"
 
-inductive_cases [elim]: "\<Gamma> \<turnstile> Var x : t"
-inductive_cases [elim]: "\<Gamma> \<turnstile> Abs t\<^sub>1 e : t"
-inductive_cases [elim]: "\<Gamma> \<turnstile> App e\<^sub>1 e\<^sub>2 : t"
-inductive_cases [elim]: "\<Gamma> \<turnstile> Rec fs : t"
-inductive_cases [elim]: "\<Gamma> \<turnstile> Proj e l : t"
-inductive_cases [elim]: "\<Gamma> \<turnstile> Inj e ts l : t"
-inductive_cases [elim]: "\<Gamma> \<turnstile> Case e cs : t"
-inductive_cases [elim]: "\<Gamma> \<turnstile>\<^sub>f [] : ts"
-inductive_cases [elim]: "\<Gamma> \<turnstile>\<^sub>f e # fs : ts"
-inductive_cases [elim]: "\<Gamma> \<turnstile>\<^sub>c [] : ts \<rightarrow> t"
-inductive_cases [elim]: "\<Gamma> \<turnstile>\<^sub>c e # cs : ts \<rightarrow> t"
+inductive_cases [elim]: "\<Delta>,\<Gamma> \<turnstile> Var x : t"
+inductive_cases [elim]: "\<Delta>,\<Gamma> \<turnstile> Abs t\<^sub>1 e : t"
+inductive_cases [elim]: "\<Delta>,\<Gamma> \<turnstile> App e\<^sub>1 e\<^sub>2 : t"
+inductive_cases [elim]: "\<Delta>,\<Gamma> \<turnstile> Rec fs : t"
+inductive_cases [elim]: "\<Delta>,\<Gamma> \<turnstile> Proj e l : t"
+inductive_cases [elim]: "\<Delta>,\<Gamma> \<turnstile> Inj e ts l : t"
+inductive_cases [elim]: "\<Delta>,\<Gamma> \<turnstile> Case e cs : t"
+inductive_cases [elim]: "\<Delta>,\<Gamma> \<turnstile> TyAbs e : t"
+inductive_cases [elim]: "\<Delta>,\<Gamma> \<turnstile> TyApp e t' : t"
+inductive_cases [elim]: "\<Delta>,\<Gamma> \<turnstile>\<^sub>f [] : ts"
+inductive_cases [elim]: "\<Delta>,\<Gamma> \<turnstile>\<^sub>f e # fs : ts"
+inductive_cases [elim]: "\<Delta>,\<Gamma> \<turnstile>\<^sub>c [] : ts \<rightarrow> t"
+inductive_cases [elim]: "\<Delta>,\<Gamma> \<turnstile>\<^sub>c e # cs : ts \<rightarrow> t"
 
-lemma canonical_arrow [simp]: "\<Gamma> \<turnstile> e : Arrow t\<^sub>1 t\<^sub>2 \<Longrightarrow> is_value e \<Longrightarrow> \<exists>e'. e = Abs t\<^sub>1 e'"
+lemma canonical_arrow [simp]: "\<Delta>,\<Gamma> \<turnstile> e : Arrow t\<^sub>1 t\<^sub>2 \<Longrightarrow> is_value e \<Longrightarrow> \<exists>e'. e = Abs t\<^sub>1 e'"
   by (induction \<Gamma> e "Arrow t\<^sub>1 t\<^sub>2" rule: typecheck_typecheck_fs_typecheck_cs.inducts(1)) simp_all
 
-lemma canonical_record [simp]: "\<Gamma> \<turnstile> e : Record ts \<Longrightarrow> is_value e \<Longrightarrow> 
-    \<exists>fs. e = Rec fs \<and> is_value_f fs \<and> \<Gamma> \<turnstile>\<^sub>f fs : ts"
+lemma canonical_record [simp]: "\<Delta>,\<Gamma> \<turnstile> e : Record ts \<Longrightarrow> is_value e \<Longrightarrow> 
+    \<exists>fs. e = Rec fs \<and> is_value_f fs \<and> \<Delta>,\<Gamma> \<turnstile>\<^sub>f fs : ts"
   by (induction \<Gamma> e "Record ts" rule: typecheck_typecheck_fs_typecheck_cs.inducts(1)) simp_all
 
-lemma canonical_variant [simp]: "\<Gamma> \<turnstile> e : Variant ts \<Longrightarrow> is_value e \<Longrightarrow> 
+lemma canonical_variant [simp]: "\<Delta>,\<Gamma> \<turnstile> e : Variant ts \<Longrightarrow> is_value e \<Longrightarrow> 
     \<exists>l e'. e = Inj l ts e' \<and> is_value e' \<and> l < length ts"
   by (induction \<Gamma> e "Variant ts" rule: typecheck_typecheck_fs_typecheck_cs.inducts(1)) auto
 
-lemma [simp]: "\<Gamma> \<turnstile>\<^sub>f fs : ts \<Longrightarrow> lookup l ts = Some t \<Longrightarrow> \<exists>e. lookup l fs = Some e"
+lemma canonical_forall [simp]: "\<Delta>,\<Gamma> \<turnstile> e : Forall t \<Longrightarrow> is_value e \<Longrightarrow> \<exists>e'. e = TyAbs e'"
+  by (induction \<Gamma> e "Forall t" rule: typecheck_typecheck_fs_typecheck_cs.inducts(1)) auto
+
+lemma [simp]: "\<Delta>,\<Gamma> \<turnstile>\<^sub>f fs : ts \<Longrightarrow> lookup l ts = Some t \<Longrightarrow> \<exists>e. lookup l fs = Some e"
   by (induction l fs arbitrary: ts rule: lookup.induct) auto
 
-lemma [simp]: "\<Gamma> \<turnstile>\<^sub>f vs : vts \<Longrightarrow> \<Gamma> \<turnstile>\<^sub>f nvs : nvts \<Longrightarrow> \<Gamma> \<turnstile>\<^sub>f vs @ nvs : vts @ nvts"
+lemma [simp]: "\<Delta>,\<Gamma> \<turnstile>\<^sub>f vs : vts \<Longrightarrow> \<Delta>,\<Gamma> \<turnstile>\<^sub>f nvs : nvts \<Longrightarrow> \<Delta>,\<Gamma> \<turnstile>\<^sub>f vs @ nvs : vts @ nvts"
   by (induction \<Gamma> vs vts rule: typecheck_typecheck_fs_typecheck_cs.inducts(2)) simp_all
 
-lemma [simp]: "\<Gamma> \<turnstile> e : t \<Longrightarrow> x \<le> length \<Gamma> \<Longrightarrow> insert_at x t' \<Gamma> \<turnstile> incr\<^sub>e\<^sub>e x e : t"
-  and [simp]: "\<Gamma> \<turnstile>\<^sub>f fs : ts \<Longrightarrow> x \<le> length \<Gamma> \<Longrightarrow> insert_at x t' \<Gamma> \<turnstile>\<^sub>f map (incr\<^sub>e\<^sub>e x) fs : ts"
-  and [simp]: "\<Gamma> \<turnstile>\<^sub>c fs : ts \<rightarrow> t \<Longrightarrow> x \<le> length \<Gamma> \<Longrightarrow> 
-    insert_at x t' \<Gamma> \<turnstile>\<^sub>c map (incr\<^sub>e\<^sub>e (Suc x)) fs : ts \<rightarrow> t"
-  by (induction \<Gamma> e t and \<Gamma> fs ts and \<Gamma> fs ts t arbitrary: x and x and x 
+lemma [simp]: "\<Delta>,\<Gamma> \<turnstile> e : t \<Longrightarrow> Suc \<Delta>,map (incr\<^sub>t\<^sub>t x) \<Gamma> \<turnstile> incr\<^sub>t\<^sub>e x e : incr\<^sub>t\<^sub>t x t"
+  and [simp]: "\<Delta>,\<Gamma> \<turnstile>\<^sub>f fs : ts \<Longrightarrow> Suc \<Delta>,map (incr\<^sub>t\<^sub>t x) \<Gamma> \<turnstile>\<^sub>f map (incr\<^sub>t\<^sub>e x) fs : map (incr\<^sub>t\<^sub>t x) ts"
+  and [simp]: "\<Delta>,\<Gamma> \<turnstile>\<^sub>c cs : ts \<rightarrow> t \<Longrightarrow>
+    Suc \<Delta>,map (incr\<^sub>t\<^sub>t x) \<Gamma> \<turnstile>\<^sub>c map (incr\<^sub>t\<^sub>e x) cs : map (incr\<^sub>t\<^sub>t x) ts \<rightarrow> incr\<^sub>t\<^sub>t x t "
+  proof (induction \<Delta> \<Gamma> e t and \<Delta> \<Gamma> fs ts and \<Delta> \<Gamma> cs ts t arbitrary: x and x and x
+         rule: typecheck_typecheck_fs_typecheck_cs.inducts) 
+  case (tc_app \<Delta> \<Gamma> e\<^sub>1 t\<^sub>1 t\<^sub>2 e\<^sub>2)
+    hence "Suc \<Delta>,map (incr\<^sub>t\<^sub>t x) \<Gamma> \<turnstile> incr\<^sub>t\<^sub>e x e\<^sub>1 : Arrow (incr\<^sub>t\<^sub>t x t\<^sub>1) (incr\<^sub>t\<^sub>t x t\<^sub>2)" by simp
+    moreover from tc_app have "Suc \<Delta>,map (incr\<^sub>t\<^sub>t x) \<Gamma> \<turnstile> incr\<^sub>t\<^sub>e x e\<^sub>2 : incr\<^sub>t\<^sub>t x t\<^sub>1" by simp
+    ultimately show ?case by simp
+  next case (tc_proj \<Delta> \<Gamma> e ts l t)
+    hence "Suc \<Delta>,map (incr\<^sub>t\<^sub>t x) \<Gamma> \<turnstile> incr\<^sub>t\<^sub>e x e : Record (map (incr\<^sub>t\<^sub>t x) ts)" by simp
+    moreover from tc_proj have "lookup l (map (incr\<^sub>t\<^sub>t x) ts) = Some (incr\<^sub>t\<^sub>t x t)" by simp
+    ultimately show ?case by simp
+  next case (tc_inj \<Delta> \<Gamma> e t l ts)
+    hence "Suc \<Delta>,map (incr\<^sub>t\<^sub>t x) \<Gamma> \<turnstile> incr\<^sub>t\<^sub>e x e : incr\<^sub>t\<^sub>t x t" by simp
+    moreover from tc_inj have "lookup l (map (incr\<^sub>t\<^sub>t x) ts) = Some (incr\<^sub>t\<^sub>t x t)" by simp
+    moreover from tc_inj have "\<forall>tt \<in> set (map (incr\<^sub>t\<^sub>t x) ts). Suc \<Delta> \<turnstile>\<^sub>k tt" by simp
+    ultimately show ?case by simp
+  next case (tc_case \<Delta> \<Gamma> e ts cs t)
+    hence "Suc \<Delta>,map (incr\<^sub>t\<^sub>t x) \<Gamma> \<turnstile> incr\<^sub>t\<^sub>e x e : Variant (map (incr\<^sub>t\<^sub>t x) ts)" by simp
+    moreover from tc_case have "Suc \<Delta>,map (incr\<^sub>t\<^sub>t x) \<Gamma> \<turnstile>\<^sub>c map (incr\<^sub>t\<^sub>e x) cs : 
+      map (incr\<^sub>t\<^sub>t x) ts \<rightarrow> incr\<^sub>t\<^sub>t x t" by simp
+    ultimately show ?case by simp
+  next case (tc_tyapp \<Delta> \<Gamma> e t t')
+    hence "Suc \<Delta>,map (incr\<^sub>t\<^sub>t x) \<Gamma> \<turnstile> incr\<^sub>t\<^sub>e x e : Forall (incr\<^sub>t\<^sub>t (Suc x) t)" by simp 
+    moreover from tc_tyapp have "Suc \<Delta> \<turnstile>\<^sub>k incr\<^sub>t\<^sub>t x t'" by simp
+    ultimately have "Suc \<Delta>,map (incr\<^sub>t\<^sub>t x) \<Gamma> \<turnstile> TyApp (incr\<^sub>t\<^sub>e x e) (incr\<^sub>t\<^sub>t x t') : 
+      subst\<^sub>t\<^sub>t 0 (incr\<^sub>t\<^sub>t x t') (incr\<^sub>t\<^sub>t (Suc x) t)"
+        by (metis typecheck_typecheck_fs_typecheck_cs.tc_tyapp)
+    thus ?case by simp
+  qed simp_all
+
+lemma tc_subst\<^sub>t\<^sub>e [simp]: "Suc \<Delta>,\<Gamma> \<turnstile> e : t \<Longrightarrow> \<Delta> \<turnstile>\<^sub>k t' \<Longrightarrow> x \<le> \<Delta> \<Longrightarrow> 
+    \<Delta>,map (subst\<^sub>t\<^sub>t x t') \<Gamma> \<turnstile> subst\<^sub>t\<^sub>e x t' e : subst\<^sub>t\<^sub>t x t' t"
+  and [simp]: "Suc \<Delta>,\<Gamma> \<turnstile>\<^sub>f fs : ts \<Longrightarrow> \<Delta> \<turnstile>\<^sub>k t' \<Longrightarrow> x \<le> \<Delta> \<Longrightarrow> 
+    \<Delta>,map (subst\<^sub>t\<^sub>t x t') \<Gamma> \<turnstile>\<^sub>f map (subst\<^sub>t\<^sub>e x t') fs : map (subst\<^sub>t\<^sub>t x t') ts"
+  and [simp]: "Suc \<Delta>,\<Gamma> \<turnstile>\<^sub>c cs : ts \<rightarrow> t \<Longrightarrow> \<Delta> \<turnstile>\<^sub>k t' \<Longrightarrow> x \<le> \<Delta> \<Longrightarrow> 
+    \<Delta>,map (subst\<^sub>t\<^sub>t x t') \<Gamma> \<turnstile>\<^sub>c map (subst\<^sub>t\<^sub>e x t') cs : map (subst\<^sub>t\<^sub>t x t') ts \<rightarrow> subst\<^sub>t\<^sub>t x t' t "
+  by (induction "Suc \<Delta>" \<Gamma> e t and "Suc \<Delta>" \<Gamma> fs ts and "Suc \<Delta>" \<Gamma> cs ts t 
+      arbitrary: \<Delta> x t' and \<Delta> x t' and \<Delta> x t'
       rule: typecheck_typecheck_fs_typecheck_cs.inducts) 
      fastforce+
 
-lemma [simp]: "insert_at x t' \<Gamma> \<turnstile> e : t \<Longrightarrow> x \<le> length \<Gamma> \<Longrightarrow> \<Gamma> \<turnstile> e' : t' \<Longrightarrow> \<Gamma> \<turnstile> subst\<^sub>e\<^sub>e x e' e : t"
-  and [simp]: "insert_at x t' \<Gamma> \<turnstile>\<^sub>f fs : ts \<Longrightarrow> x \<le> length \<Gamma> \<Longrightarrow> \<Gamma> \<turnstile> e' : t' \<Longrightarrow> 
-    \<Gamma> \<turnstile>\<^sub>f map (subst\<^sub>e\<^sub>e x e') fs : ts"
-  and [simp]: "insert_at x t' \<Gamma> \<turnstile>\<^sub>c fs : ts \<rightarrow> t \<Longrightarrow> x \<le> length \<Gamma> \<Longrightarrow> \<Gamma> \<turnstile> e' : t' \<Longrightarrow> 
-    \<Gamma> \<turnstile>\<^sub>c map (subst\<^sub>e\<^sub>e (Suc x) (incr\<^sub>e\<^sub>e 0 e')) fs : ts \<rightarrow> t "
-  proof (induction "insert_at x t' \<Gamma>" e t and "insert_at x t' \<Gamma>" fs ts 
-               and "insert_at x t' \<Gamma>" fs ts t 
-         arbitrary: \<Gamma> x e' and \<Gamma> x e' and \<Gamma> x e'
+lemma [simp]: "\<Delta>,\<Gamma> \<turnstile> e : t \<Longrightarrow> x \<le> length \<Gamma> \<Longrightarrow> \<Delta>,insert_at x t' \<Gamma> \<turnstile> incr\<^sub>e\<^sub>e x e : t"
+  and [simp]: "\<Delta>,\<Gamma> \<turnstile>\<^sub>f fs : ts \<Longrightarrow> x \<le> length \<Gamma> \<Longrightarrow> \<Delta>,insert_at x t' \<Gamma> \<turnstile>\<^sub>f map (incr\<^sub>e\<^sub>e x) fs : ts"
+  and [simp]: "\<Delta>,\<Gamma> \<turnstile>\<^sub>c cs : ts \<rightarrow> t \<Longrightarrow> x \<le> length \<Gamma> \<Longrightarrow> 
+    \<Delta>,insert_at x t' \<Gamma> \<turnstile>\<^sub>c map (incr\<^sub>e\<^sub>e (Suc x)) cs : ts \<rightarrow> t"
+  proof (induction \<Delta> \<Gamma> e t and \<Delta> \<Gamma> fs ts and \<Delta> \<Gamma> cs ts t arbitrary: x t' and x t' and x t'
+         rule: typecheck_typecheck_fs_typecheck_cs.inducts) 
+  case (tc_app \<Delta> \<Gamma> e\<^sub>1 t\<^sub>1 t\<^sub>2 e\<^sub>2)
+    hence "\<Delta>,insert_at x t' \<Gamma> \<turnstile> incr\<^sub>e\<^sub>e x e\<^sub>1 : Arrow t\<^sub>1 t\<^sub>2" by simp
+    moreover from tc_app have "\<Delta>,insert_at x t' \<Gamma> \<turnstile> incr\<^sub>e\<^sub>e x e\<^sub>2 : t\<^sub>1" by simp
+    ultimately show ?case by simp
+  next case (tc_proj \<Delta> \<Gamma> e ts l t)
+    hence "\<Delta>,insert_at x t' \<Gamma> \<turnstile> incr\<^sub>e\<^sub>e x e : Record ts" by simp
+    moreover from tc_proj have "lookup l ts = Some t" by simp
+    ultimately show ?case by simp
+  next case (tc_inj \<Delta> \<Gamma> e t l ts)
+    hence "\<Delta>,insert_at x t' \<Gamma> \<turnstile> incr\<^sub>e\<^sub>e x e : t" by simp
+    moreover from tc_inj have "lookup l ts = Some t" by simp
+    moreover from tc_inj have "\<forall>tt \<in> set ts. \<Delta> \<turnstile>\<^sub>k tt" by simp
+    ultimately show ?case by simp
+  next case (tc_case \<Delta> \<Gamma> e ts cs t)
+    hence "\<Delta>,insert_at x t' \<Gamma> \<turnstile> incr\<^sub>e\<^sub>e x e : Variant ts " by simp
+    moreover from tc_case have "\<Delta>,insert_at x t' \<Gamma> \<turnstile>\<^sub>c map (incr\<^sub>e\<^sub>e (Suc x)) cs : ts \<rightarrow> t" by simp
+    ultimately show ?case by simp
+  qed simp_all
+
+lemma [simp]: "\<Delta>,insert_at x t' \<Gamma> \<turnstile> e : t \<Longrightarrow> x \<le> length \<Gamma> \<Longrightarrow> \<Delta>,\<Gamma> \<turnstile> e' : t' \<Longrightarrow> \<Delta>,
+    \<Gamma> \<turnstile> subst\<^sub>e\<^sub>e x e' e : t"
+  and [simp]: "\<Delta>,insert_at x t' \<Gamma> \<turnstile>\<^sub>f fs : ts \<Longrightarrow> x \<le> length \<Gamma> \<Longrightarrow> \<Delta>,\<Gamma> \<turnstile> e' : t' \<Longrightarrow> 
+    \<Delta>,\<Gamma> \<turnstile>\<^sub>f map (subst\<^sub>e\<^sub>e x e') fs : ts"
+  and [simp]: "\<Delta>,insert_at x t' \<Gamma> \<turnstile>\<^sub>c fs : ts \<rightarrow> t \<Longrightarrow> x \<le> length \<Gamma> \<Longrightarrow> \<Delta>,\<Gamma> \<turnstile> e' : t' \<Longrightarrow> 
+    \<Delta>,\<Gamma> \<turnstile>\<^sub>c map (subst\<^sub>e\<^sub>e (Suc x) (incr\<^sub>e\<^sub>e 0 e')) fs : ts \<rightarrow> t "
+  proof (induction \<Delta> "insert_at x t' \<Gamma>" e t and \<Delta> "insert_at x t' \<Gamma>" fs ts 
+               and \<Delta> "insert_at x t' \<Gamma>" fs ts t 
+         arbitrary: \<Gamma> x e' t' and \<Gamma> x e' t' and \<Gamma> x e' t'
          rule: typecheck_typecheck_fs_typecheck_cs.inducts)
   case (tc_var y t)
     thus ?case by (cases y) auto
   qed fastforce+
 
-lemma [elim]: "\<Gamma> \<turnstile>\<^sub>f fs : ts \<Longrightarrow> lookup l fs = Some e \<Longrightarrow> lookup l ts = Some t \<Longrightarrow> \<Gamma> \<turnstile> e : t" 
+lemma [elim]: "\<Delta>,\<Gamma> \<turnstile>\<^sub>f fs : ts \<Longrightarrow> lookup l fs = Some e \<Longrightarrow> lookup l ts = Some t \<Longrightarrow> \<Delta>,\<Gamma> \<turnstile> e : t" 
   by (induction l fs arbitrary: ts rule: lookup.induct) auto
 
-lemma [elim]: "\<Gamma> \<turnstile>\<^sub>c cs : ts \<rightarrow> t \<Longrightarrow> lookup l cs = Some e \<Longrightarrow> lookup l ts = Some t' \<Longrightarrow> 
-    insert_at 0 t' \<Gamma> \<turnstile> e : t" 
+lemma [elim]: "\<Delta>,\<Gamma> \<turnstile>\<^sub>c cs : ts \<rightarrow> t \<Longrightarrow> lookup l cs = Some e \<Longrightarrow> lookup l ts = Some t' \<Longrightarrow> 
+    \<Delta>,insert_at 0 t' \<Gamma> \<turnstile> e : t" 
   by (induction l cs arbitrary: ts rule: lookup.induct) auto
 
 end
