Evaluate.thy
@@ -6,19 +6,21 @@ inductive reduce :: "expr \<Rightarrow> expr \<Rightarrow> bool" (infix "\<leads
   ev_beta [simp]: "is_value e\<^sub>2 \<Longrightarrow> App (Abs t e\<^sub>1) e\<^sub>2 \<leadsto>\<^sub>\<beta> subst\<^sub>e\<^sub>e 0 e\<^sub>2 e\<^sub>1" 
 | ev_proj [simp]: "is_value_f fs \<Longrightarrow> lookup l fs = Some e \<Longrightarrow> Proj (Rec fs) l \<leadsto>\<^sub>\<beta> e" 
 | ev_case [simp]: "is_value e \<Longrightarrow> lookup l cs = Some e' \<Longrightarrow> Case (Inj l ts e) cs \<leadsto>\<^sub>\<beta> subst\<^sub>e\<^sub>e 0 e e'" 
+| ev_tbeta [simp]: "TyApp (TyAbs e) t \<leadsto>\<^sub>\<beta> subst\<^sub>t\<^sub>e 0 t e" 
 
 inductive evaluate :: "expr \<Rightarrow> expr \<Rightarrow> bool" (infix "\<leadsto>" 60) where
   ev_stack [simp]: "unfold e = (s, r) \<Longrightarrow> r \<leadsto>\<^sub>\<beta> r' \<Longrightarrow> e \<leadsto> fold s r'"
 
 inductive_cases [elim]: "e \<leadsto> e'"
 
-theorem [simp]: "[] \<turnstile> e : t \<Longrightarrow> unfold e = (s, r) \<Longrightarrow> is_value e \<or> (\<exists>r'. r \<leadsto>\<^sub>\<beta> r')"
-    and "[] \<turnstile>\<^sub>f fs : ts \<Longrightarrow> \<not> is_value_f fs \<Longrightarrow> unfold_f fs = (vs, nvs, s, r) \<Longrightarrow> \<exists>r'. r \<leadsto>\<^sub>\<beta> r'"
-    and "[] \<turnstile>\<^sub>c cs : ts \<rightarrow> t \<Longrightarrow> l < length ts \<Longrightarrow> \<exists>c. lookup l cs = Some c"
-  proof (induction "[] :: type list" e t and "[] :: type list" fs ts and "[] :: type list" cs ts t
+theorem [simp]: "\<Delta>,[] \<turnstile> e : t \<Longrightarrow> unfold e = (s, r) \<Longrightarrow> is_value e \<or> (\<exists>r'. r \<leadsto>\<^sub>\<beta> r')"
+    and "\<Delta>,[] \<turnstile>\<^sub>f fs : ts \<Longrightarrow> \<not> is_value_f fs \<Longrightarrow> unfold_f fs = (vs, nvs, s, r) \<Longrightarrow> \<exists>r'. r \<leadsto>\<^sub>\<beta> r'"
+    and "\<Delta>,[] \<turnstile>\<^sub>c cs : ts \<rightarrow> t \<Longrightarrow> l < length ts \<Longrightarrow> \<exists>c. lookup l cs = Some c"
+  proof (induction \<Delta> "[] :: type list" e t and \<Delta> "[] :: type list" fs ts 
+               and \<Delta> "[] :: type list" cs ts t
          arbitrary: s r and vs nvs s r and l
          rule: typecheck_typecheck_fs_typecheck_cs.inducts)
-  case (tc_app e\<^sub>1 t\<^sub>1 t\<^sub>2 e\<^sub>2)
+  case (tc_app \<Delta> e\<^sub>1 t\<^sub>1 t\<^sub>2 e\<^sub>2)
     thus ?case
       proof (cases "is_value e\<^sub>1")
       case True note T = True
@@ -29,16 +31,16 @@ theorem [simp]: "[] \<turnstile> e : t \<Longrightarrow> unfold e = (s, r) \<Lon
             ultimately show ?thesis using ev_beta by blast
           qed (auto split: prod.splits)
       qed (auto split: prod.splits)
-  next case (tc_proj e ts l t)
+  next case (tc_proj \<Delta> e ts l t)
     thus ?case 
       proof (cases "is_value e")
       case True
-        with tc_proj obtain fs where "r = Proj (Rec fs) l \<and> is_value_f fs \<and> [] \<turnstile>\<^sub>f fs : ts" 
+        with tc_proj obtain fs where "r = Proj (Rec fs) l \<and> is_value_f fs \<and> \<Delta>,[] \<turnstile>\<^sub>f fs : ts" 
           by fastforce
         moreover with tc_proj obtain r' where "lookup l fs = Some r'" by fastforce
         ultimately show ?thesis using ev_proj by blast
       qed (auto split: prod.splits)
-  next case (tc_case e ts cs t)
+  next case (tc_case \<Delta> e ts cs t)
     thus ?case
       proof (cases "is_value e")
       case True
@@ -47,13 +49,21 @@ theorem [simp]: "[] \<turnstile> e : t \<Longrightarrow> unfold e = (s, r) \<Lon
         moreover with tc_case obtain r' where "lookup l cs = Some r'" by fastforce
         ultimately show ?thesis using ev_case by blast
       qed (auto split: prod.splits)
+  next case (tc_tyapp \<Delta> e t t')
+    thus ?case
+      proof (cases "is_value e")
+      case True
+        with tc_tyapp obtain e' where "e = TyAbs e'" by fastforce
+        with tc_tyapp True have "r \<leadsto>\<^sub>\<beta> subst\<^sub>t\<^sub>e 0 t' e'" by fastforce
+        thus ?thesis by fastforce
+      qed (auto split: prod.splits)
   next case (tcc_cons t' e t fs ts)
     thus ?case by (induction l) simp_all
   qed (auto split: if_splits prod.splits)
 
-theorem progress: "[] \<turnstile> e : t \<Longrightarrow> is_value e \<or> (\<exists>e'. e \<leadsto> e')"
+theorem progress: "\<Delta>,[] \<turnstile> e : t \<Longrightarrow> is_value e \<or> (\<exists>e'. e \<leadsto> e')"
   proof -
-    assume "[] \<turnstile> e : t"
+    assume "\<Delta>,[] \<turnstile> e : t"
     moreover obtain s r where S: "unfold e = (s, r)" by fastforce
     ultimately have R: "is_value e \<or> (\<exists>r'. r \<leadsto>\<^sub>\<beta> r')" by simp
     thus "is_value e \<or> (\<exists>e'. e \<leadsto> e')" 
@@ -63,19 +73,24 @@ theorem progress: "[] \<turnstile> e : t \<Longrightarrow> is_value e \<or> (\<e
       qed simp_all
   qed
 
-lemma preservation\<^sub>\<beta>: "e \<leadsto>\<^sub>\<beta> e' \<Longrightarrow> \<Gamma> \<turnstile> e : t \<Longrightarrow> \<Gamma> \<turnstile> e' : t"
+lemma preservation\<^sub>\<beta>: "e \<leadsto>\<^sub>\<beta> e' \<Longrightarrow> \<Delta>,\<Gamma> \<turnstile> e : t \<Longrightarrow> \<Delta>,\<Gamma> \<turnstile> e' : t"
   proof (induction e e' rule: reduce.induct) 
   case (ev_case e l cs e' ts)
-    then obtain t' where "(\<Gamma> \<turnstile> e : t') \<and> lookup l ts = Some t' \<and> \<Gamma> \<turnstile>\<^sub>c cs : ts \<rightarrow> t" by fastforce
-    moreover with ev_case have "insert_at 0 t' \<Gamma> \<turnstile> e' : t" by fastforce
+    then obtain t' where "(\<Delta>,\<Gamma> \<turnstile> e : t') \<and> lookup l ts = Some t' \<and> \<Delta>,\<Gamma> \<turnstile>\<^sub>c cs : ts \<rightarrow> t" by fastforce
+    moreover with ev_case have "\<Delta>,insert_at 0 t' \<Gamma> \<turnstile> e' : t" by fastforce
     ultimately show ?case by simp
+  next case (ev_tbeta e t')
+    then obtain tt where "(Suc \<Delta>,map (incr\<^sub>t\<^sub>t 0) \<Gamma> \<turnstile> e : tt) \<and> (\<Delta> \<turnstile>\<^sub>k t') \<and> t = subst\<^sub>t\<^sub>t 0 t' tt" 
+      by fastforce
+    hence "\<Delta>,map (subst\<^sub>t\<^sub>t 0 t') (map (incr\<^sub>t\<^sub>t 0) \<Gamma>) \<turnstile> subst\<^sub>t\<^sub>e 0 t' e : t" using tc_subst\<^sub>t\<^sub>e by blast
+    thus ?case by simp
   qed fastforce+
 
-theorem preservation: "e \<leadsto> e' \<Longrightarrow> \<Gamma> \<turnstile> e : t \<Longrightarrow> \<Gamma> \<turnstile> e' : t"
+theorem preservation: "e \<leadsto> e' \<Longrightarrow> \<Delta>,\<Gamma> \<turnstile> e : t \<Longrightarrow> \<Delta>,\<Gamma> \<turnstile> e' : t"
   proof (induction e e' rule: evaluate.induct)
   case (ev_stack e s r r')
-    then obtain t' where "(\<Gamma> \<turnstile>\<^sub>s s : t' \<rightarrow> t) \<and> \<Gamma> \<turnstile> r : t'" by fastforce
-    moreover with ev_stack have "\<Gamma> \<turnstile> r' : t'" using preservation\<^sub>\<beta> by simp
+    then obtain t' where "(\<Delta>,\<Gamma> \<turnstile>\<^sub>s s : t' \<rightarrow> t) \<and> \<Delta>,\<Gamma> \<turnstile> r : t'" by fastforce
+    moreover with ev_stack have "\<Delta>,\<Gamma> \<turnstile> r' : t'" using preservation\<^sub>\<beta> by simp
     ultimately show ?case by fastforce
   qed
 
